theories/heap_lang/locations.v
@@ -1,0 +1,44 @@
+From iris.algebra Require Import base.
+From stdpp Require Import countable numbers gmap.
+
+Record loc := { loc_car : Z }.
+
+Instance loc_eq_decision : EqDecision loc.
+Proof. solve_decision. Qed.
+
+Instance loc_inhabited : Inhabited loc := populate {|loc_car := 0 |}.
+
+Instance loc_countable : Countable loc.
+Proof. by apply (inj_countable' loc_car (λ i, {| loc_car := i |})); intros []. Qed.
+
+Definition loc_add (l : loc) (off : Z) : loc :=
+  {| loc_car := loc_car l + off|}.
+
+Notation "l +ₗ off" := (loc_add l off) (at level 50, left associativity).
+
+Lemma loc_add_assoc l i j : l +ₗ i +ₗ j = l +ₗ (i + j).
+Proof. destruct l; rewrite /loc_add /=; f_equal; lia. Qed.
+
+Lemma loc_add_0 l : l +ₗ 0 = l.
+Proof. destruct l; rewrite /loc_add /=; f_equal; lia. Qed.
+
+Instance loc_add_inj l : Inj eq eq (loc_add l).
+Proof. destruct l; rewrite /Inj /loc_add /=; intros; simplify_eq; lia. Qed.
+
+Definition fresh_locs (g : gset loc) (n : Z) : loc :=
+  {| loc_car := set_fold (λ k r, (1 + loc_car k) `max` r)%Z 1%Z g |}.
+
+Lemma fresh_locs_fresh g n i :
+  (0 ≤ i)%Z → (i < n)%Z → (fresh_locs g n) +ₗ i ∉ g.
+Proof.
+  rewrite /fresh_locs /loc_add /=; intros Hil _ Hf; clear n.
+  cut (∀ x, x ∈ g →
+            loc_car x < set_fold (λ k r, ((1 + loc_car k) `max` r)%Z) 1%Z g)%Z.
+  { intros Hlem; apply Hlem in Hf; simpl in *; lia. }
+  clear Hf.
+  eapply (set_fold_ind_L
+            (λ z g, ∀ x : loc, x ∈ g → (loc_car x < z)%Z));
+    try set_solver by eauto with lia.
+Qed.
+
+Global Opaque fresh_locs.
